on inst case

wip/formalization/Problems.v
@@ -46,6 +46,14 @@ Fixpoint lhvars_Probl (P : Problem) : set SortedVar :=
   | (equ_s σ τ) :: P0 => set_union sortedvar_eqdec (vars_of_sexp σ) (lhvars_Probl P0)                     
   end.  
 
+Fixpoint rhvars_Probl (P : Problem) : set SortedVar :=
+  match P with
+  | [] => []
+  | (equ s t) :: P0 => set_union sortedvar_eqdec (vars_of_exp t) (rhvars_Probl P0)
+  | (equ_s σ τ) :: P0 => set_union sortedvar_eqdec (vars_of_sexp τ) (rhvars_Probl P0)                     
+  end.  
+
+
 Fixpoint Problem_vars (P : Problem) : set SortedVar :=
   match P with
     | [] => []
@@ -59,4 +67,100 @@ Notation "P \ u" := (set_remove Equation_eqdec u P) (at level 67).
 Notation "P |+ u" := (set_add Equation_eqdec u P) (at level 67).
 Notation "P |^^ S" := (subs_Problem_right P S) (at level 67).
 
+
+Lemma in_exp_then_in_left_problem : forall P s t V, set_In V (vars_of_exp s) ->
+                                               set_In (equ s t) P -> 
+                                               set_In V (lhvars_Probl P).
+Proof.
+  intro P.
+  induction P; intros.
+  - now simpl in *.
+  - simpl in *.
+    destruct V as [X | Y]; destruct a as [s' t' | σ τ].
+     1,3 : destruct H0;
+           [inversion H0; subst;
+            now apply set_union_intro1 |
+            apply set_union_intro2;
+            eapply IHP; eauto].
+     1,2 : destruct H0;
+           [ inversion H0 |
+             apply set_union_intro2;
+             eapply IHP; eauto].
+Qed.
+
+Lemma in_sexp_then_in_left_problem : forall P σ τ V, set_In V (vars_of_sexp σ) ->
+                                               set_In (equ_s σ τ) P -> 
+                                               set_In V (lhvars_Probl P).
+Proof.
+  intro P.
+  induction P; intros.
+  - now simpl in *.
+  - simpl in *.
+    destruct V as [X | Y]; destruct a as [s t | σ' τ'].
+    1,3 : destruct H0;
+           [ inversion H0 |
+             apply set_union_intro2;
+             eapply IHP; eauto].
+    1,2 :  destruct H0;
+           [inversion H0; subst;
+            now apply set_union_intro1 |
+            apply set_union_intro2;
+            eapply IHP; eauto].
+Qed.
+
+Lemma in_left_problem_then_in_problem : forall P V, set_In V (lhvars_Probl P) ->
+                                               set_In V (Problem_vars P).
+Proof.
+  intros P.
+  induction P; intros; simpl in *; trivial.
+  destruct V as [X | Y]; destruct a as [s t | σ τ].
+   all :apply set_union_elim in H; destruct H;
+       [now apply set_union_intro1 |
+       apply set_union_intro2; apply set_union_intro2; now apply IHP].
+Qed.
+
+
+
+Lemma in_exp_then_in_right_problem : forall P s t V, set_In V (vars_of_exp t) ->
+                                               set_In (equ s t) P -> 
+                                               set_In V (rhvars_Probl P).
+Admitted.
+
+Lemma in_sexp_then_in_right_problem : forall P σ τ V, set_In V (vars_of_sexp τ) ->
+                                               set_In (equ_s σ τ) P -> 
+                                               set_In V (rhvars_Probl P).
+Admitted.
+
+
+
+Lemma in_right_problem_then_in_problem : forall P V, set_In V (rhvars_Probl P) ->
+                                               set_In V (Problem_vars P).
+Admitted.
+
+
+
+
+Lemma push_subst_problem_exp : forall s t S P, set_In (equ s t) P -> set_In (equ s (sub t S)) (P |^^ S).
+Proof.
+  intros.
+  induction P.
+  - destruct H.
+  - simpl in *; subst.
+    destruct H.
+    + rewrite H.
+      simpl. now left.
+    + destruct a; simpl; right; now apply IHP.
+Qed.     
+
+Lemma push_subst_problem_sexp : forall σ τ S P, set_In (equ_s σ τ) P -> set_In (equ_s σ (sub_s τ S)) (P |^^ S).
+Proof.
+  intros.
+  induction P.
+  - destruct H.
+  - simpl in *; subst.
+    destruct H.
+    + rewrite H.
+      simpl. now left.
+    + destruct a; simpl; right; now apply IHP.
+Qed.
 
