wip/formalization/Soundness.v
@@ -23,7 +23,7 @@ Lemma match_sol_preservation : forall Sl T T',
 
       valid_tuple T ->
 
-      set_inter sortedvar_eqdec (lhvars_Probl (snd T)) (dom_rec Sl) = [] ->
+      set_inter sortedvar_eqdec (dom_rec Sl)  (lhvars_Probl (snd T)) = [] ->
 
       smatch T T' ->
 
@@ -55,13 +55,55 @@ Proof.
   - admit.
   - admit.
   - admit.
-
   (* Inst Exp Case *)
   - unfold subs_equiv in HEq3; destruct HEq3 as [HEq3 HEq3'].   
     destruct (Equation_eqdec (equ s0 t0) (equ s (VarExp X))) as [Eq | Eq]; intros.
     + rewrite Eq in *. simpl in *.
       inversion Eq; subst. clear Eq.
       simpl. apply σmin_equiv_trans with (t := sub s S'').
+      apply (proj1 not_in_dom_same_exp); split; intros.      
+      eapply σmin_comp_prop_exp with (S:= sub_comp S ([exp_assign X s])%list).
+      eapply set_nocommon_inter_forall_flip with (X:= exp_var X0) in HVl.
+      apply In_dom_eq_dom_flip_exp. apply not_In_dom_lookup_flip_exp.
+      apply not_in_dom_lookup_same_exp in HVl.
+      rewrite look_up_sub_comp_exp. rewrite HVl. simpl.
+      destruct (var_eqdec X X0); subst.
+      eapply in_exp_then_in_left_problem with (P := P) in H1. contradiction. apply HinP. trivial.
+      eapply in_exp_then_in_left_problem with (P := P) in H1.
+      now apply in_left_problem_then_in_problem. apply HinP.
+      eapply set_nocommon_inter_forall_flip in HLh.
+      apply HLh. eapply in_exp_then_in_left_problem. apply H1. apply H0.
+      unfold subs_equiv; split; eauto. 
+
+      eapply σmin_comp_prop_sexp with (S:= sub_comp S ([exp_assign X s])%list).
+      eapply set_nocommon_inter_forall_flip with (X := sexp_var Y) in HVl.
+      apply In_dom_eq_dom_flip_sexp. apply not_In_dom_lookup_flip_sexp.
+      apply not_in_dom_lookup_same_sexp in HVl.
+      rewrite look_up_sub_comp_sexp.  rewrite HVl. now simpl.
+      eapply in_exp_then_in_left_problem with (P := P) in H1. 
+      now apply in_left_problem_then_in_problem. apply HinP. 
+      eapply set_nocommon_inter_forall_flip in HLh.
+      apply HLh. eapply in_exp_then_in_left_problem. apply H1. apply H0.
+      unfold subs_equiv; split; eauto.
+
+      specialize (HEq3 X).
+      rewrite look_up_sub_comp_exp in HEq3. rewrite in_subcomp_second_arg_exp in HEq3.
+      simpl in HEq3. destruct (var_eqdec X X); [assumption | contradiction].
+      eapply set_nocommon_inter_forall_flip with (X:= exp_var X) in HVl.
+      apply HVl. eapply in_right_problem_then_in_problem.
+      eapply in_exp_then_in_right_problem.
+      2: apply H0. now left.
+   +  destruct (set_In_dec sortedvar_eqdec (exp_var X) (vars_of_exp t0)) as [Ht0 | Hnt0].
+      apply σmin_equiv_trans with (t  := sub t0 (sub_comp ([exp_assign X s]) Sl)).
+      rewrite (proj1 subst_comp_expand).
+      apply HEq1. apply push_subst_problem_exp.
+      now apply set_remove_3.
+
+      
+       
+      
       
 
+      
+     
 Admitted.      
